projectVampire/dafny/hospital.dfy
@@ -1,0 +1,88 @@
+class hospital {
+
+	var x : int;
+	var y : int;
+	var name : string;
+	var tMan : transportationManager;
+	var blood : array<Blood>;	
+	var size: int;
+	var available: int;	
+	var patho : pathology;
+	
+
+	predicate method Valid()
+	reads this;
+	reads this.blood;
+	requires blood != null;
+	{
+		blood != null &&
+		size > 0 &&
+		size == blood.Length &&
+		-1 < available <= size -1
+	}
+
+	method init(nm:string, xVal:int, yVal:int) 
+	modifies this
+	modifies this`x
+	modifies this`y
+	modifies this`name
+	modifies this.blood
+	modifies this`size
+	modifies this`available
+	{
+		name := nm;
+		x := xVal;
+		y := yVal;
+		size := 10;
+		available := 0;	
+		blood := new Blood[size];
+	}
+
+	method collect_blood(donordb: map<int,int>, donor_id: int, curr_time: int) 
+	modifies this.blood
+	modifies this`available
+	requires patho != null
+	requires blood != null
+	requires forall x :: 0 <= x < blood.Length && blood[x] != null ==> blood[x].state == verified
+	requires Valid();ensures Valid();
+	ensures blood[available] != null ==> blood[available].state == verified
+	ensures 0 <= available < blood.Length
+	{
+		if donor_id in donordb {
+			// do something
+		}
+		var allowed := true; // determined by value in donor class
+		if (allowed) {
+			var bld := new Blood(1); // blood as collected from donor class
+			patho.verify(bld);
+			if bld.state == verified {
+				available := if available == size -1 then 0 else available + 1;
+				blood[available] := bld;
+			}
+
+		} else {
+			// Can't take blood, too soon since last donation time
+		}
+	}
+
+	method obtainBlood()
+	modifies this.blood
+	requires blood != null
+	requires Valid();
+	ensures blood != null
+	ensures Valid()
+	ensures forall x :: 0 <= x < blood.Length ==> blood[x] == null
+	{	
+		var toSend := blood;
+		// toSend is sent to transport on dispatch request
+		var i := 0;
+		while (i < blood.Length) 
+		invariant 0 <= i <= blood.Length
+		invariant forall x :: 0 <= x < i ==> blood[x] == null;
+		{
+			blood[i] := null;
+			i := i + 1;
+		}
+	}
+
+}
