projectVampire/dafny/pathology.dfy
@@ -1,0 +1,59 @@
+class pathology {
+	
+
+	var tMan: transportationManager;
+	
+	method Init(t : transportationManager)
+	modifies this
+	modifies tMan
+	//ensures fresh(tMan)
+	{
+		tMan := t;
+	}
+	
+	
+	method accept (bld : Blood)
+	modifies tMan
+	modifies tMan.toDest
+	modifies tMan.toSend
+	modifies tMan`locale
+	modifies bld
+	requires this.tMan != null
+
+	requires tMan.toSend != null
+	requires tMan.toDest != null
+	requires forall x :: 0 <= x < tMan.toSend.Length ==> tMan.toSend[x] != bld
+	requires tMan.Valid()
+	requires bld != null
+	requires bld.state == unverified
+	ensures tMan != null
+	{
+		verify(bld);
+		if (bld.state == verified) {
+			// do something
+			tMan.receive(bld, 1); // system will find a suitable dest for blood
+			tMan.dispatchBlood();
+		} else {
+			// blood is discarded and not sent further
+		}
+	
+
+	}
+
+	method verify(bld:Blood) 
+	modifies bld
+	requires bld != null
+	requires bld.state == unverified
+	ensures bld.state == verified || bld.state == unsafe 
+	ensures bld.blood_type == O || bld.blood_type == A || bld.blood_type == AB || bld.blood_type == B
+	ensures bld.rhesus == false || bld.rhesus == true
+	ensures bld != null
+	{
+		var bType := O; // practically will be any blood_type as per blood class limits
+		var chosenRhes := false; // practically will be 0 or 1
+		var accepted := true;
+
+		bld.verify_blood(1,accepted,bType,chosenRhes);
+
+	}
+}
